Isabelle2/MultiPaxos4.thy
@@ -56,7 +56,6 @@ value "{0, 1, 2} = {1, 0, 2}"
 record 'v acc_state =
   id :: acc
   leader :: "bool"
-  acceptors :: "acc fset"
     -- {* The set of all acceptors *}
 
   ballot :: "bal option"
@@ -66,9 +65,9 @@ record 'v acc_state =
     -- {* The last vote cast by an acceptor, for each instance *}
   last_ballot :: "inst \<Rightarrow>f bal option"
     -- {* For an acceptor a, this is the ballot in which "vote a" was cast, for each instance *}
-  onebs :: "bal \<Rightarrow>f inst \<Rightarrow>f (acc \<times> ('v cmd \<times> bal) option) list"
+  onebs :: "bal \<Rightarrow>f inst \<Rightarrow>f (acc \<times> ('v cmd \<times> bal) option) set"
     -- {* For an acceptor a and a ballot b, lists of 1b-message descriptions, indexed by ballot then instance. *}
-  twobs :: "inst \<Rightarrow>f bal \<Rightarrow>f acc list"
+  twobs :: "inst \<Rightarrow>f bal \<Rightarrow>f acc set"
     -- {* For an acceptor a: lists describing the 2b messages, indexed by instance then ballot. *}
 
   next_inst :: "nat"
@@ -78,17 +77,14 @@ record 'v acc_state =
 
   commit_buffer :: "inst \<Rightarrow>f 'v cmd option"
   last_committed :: "inst"
-
-  snapshot_reference :: "inst"
-  snapshot_proposal :: "inst list"
   
 fun accs where
-  "accs (0::nat) = {||}"
-| "accs (Suc n) = (accs n) |\<union>| {|n|}"
+  "accs (0::nat) = []"
+| "accs (Suc n) = append (accs n) [n]"
 
 definition nr where
   -- {* The number of replicas *}
-  "nr s \<equiv> fcard (acceptors s)"
+  "nr acceptors \<equiv> card acceptors"
 
 text {* A few functions to export to Scala for use by the runtime. *}
 
@@ -97,32 +93,29 @@ definition get_ballot where "get_ballot s \<equiv> ballot s"
 definition is_leader where "is_leader s \<equiv> leader s"
 
 definition get_leader where 
-  "get_leader s \<equiv> case ballot s of Some (b::nat) \<Rightarrow> Some (b mod (nr s)) | _ \<Rightarrow> None"
+  "get_leader s nas \<equiv> case ballot s of Some (b::nat) \<Rightarrow> Some (b mod nas) | _ \<Rightarrow> None"
 
 definition get_next_instance where
   "get_next_instance s \<equiv> next_inst s"
-definition init_acc_state :: "nat \<Rightarrow> acc \<Rightarrow> 'v acc_state" where
-  "init_acc_state n a \<equiv> \<lparr>
+
+definition init_acc_state :: "acc \<Rightarrow> 'v acc_state" where
+  "init_acc_state a \<equiv> \<lparr>
     id = a,
     leader = False,
-    acc_state.acceptors = accs n,
 
     ballot = None,
     decided = K$ None,
     vote = K$ None, 
     last_ballot = K$ None,
-    onebs = K$ K$ [],
-    twobs = K$ K$ [],
+    onebs = K$ K$ {},
+    twobs = K$ K$ {},
 
     next_inst = 1, (* instances start at 1 *)
     last_decision = None,
     working_instances =  K$ 0,
 
     commit_buffer =  K$ None,
-    last_committed = 0,
-
-    snapshot_reference=0,
-    snapshot_proposal = []
+    last_committed = 0
    \<rparr>" 
 
 subsection {* Event handlers *}
@@ -130,10 +123,9 @@ subsection {* Event handlers *}
 text {* If we had finfun_Ex we could do this better.
   Here we use instance 0 by default, but that's arbitrary. *}
 definition one_b_quorum_received where
-  "one_b_quorum_received b s \<equiv> 
-    let at_b = onebs s $ b;
-        at_b_i = at_b $ 0
-    in 2 * length at_b_i > nr s"
+  "one_b_quorum_received b s nas \<equiv> 
+    let at_b_i = onebs s $ b $ 0
+    in 2 * card at_b_i > nas"
 
 fun getOwnedBallot where 
   "getOwnedBallot a (Suc b) N = (if ((Suc b) mod N = a) then (Suc b)
@@ -149,49 +141,50 @@ fun nx_bal where
 | "nx_bal a (Some b) N = suc_bal a b N"
 
 definition leader_of_bal where
-  "leader_of_bal s b \<equiv> case b of None \<Rightarrow> 0 | Some b \<Rightarrow>
-    (b mod (nr s))"
+  "leader_of_bal s b nas \<equiv> case b of None \<Rightarrow> 0 | Some b \<Rightarrow>
+    (b mod nas)"
 
-definition send_all where "send_all s a m \<equiv> fimage (\<lambda> a2 . Packet (id s) a2 m)  (acceptors s |-| {|a|})"
+definition send_all where "send_all state acc ms acceptors \<equiv> image (\<lambda> a2 . Packet (id state) a2 ms)  (acceptors - {acc})"
 
 definition do_2a where
-  "do_2a s v \<equiv>
+  "do_2a s v acceptors \<equiv>
     let
       a = id s;
       inst = (next_inst s);
       b = the (ballot s);
       msg = Phase2a inst b v a;
       new_state = s\<lparr>next_inst := (inst+1),
-        twobs := finfun_update_code (twobs s) inst ((K$ [])(b $:= [a])),
+        twobs := finfun_update_code (twobs s) inst ((K$ {})(b $:= {a})),
         working_instances := (working_instances s)(inst $:=1) (* Added by ian to track working instances *)
        \<rparr>
     in
-      (new_state, send_all s a msg)"
+      (new_state, send_all s a msg acceptors)"
 
-definition propose :: "'v \<Rightarrow> 'v acc_state \<Rightarrow> ('v acc_state \<times> 'v packet fset)" where
+definition propose :: "'v \<Rightarrow> 'v acc_state \<Rightarrow> nat \<Rightarrow> acc set \<Rightarrow> ('v acc_state \<times> 'v packet set)" where
   -- {* If leader, then go ahead with 2a, otherwise forward to the leader. *}
-  "propose v s \<equiv> let a = id s in
-    (if (leader_of_bal s (ballot s) = a \<and> leader s)
-      then do_2a s (Cmd v)
-      else ( if (leader_of_bal s (ballot s) = a)
-        then (s,{||}) (* TODO: here we loose the proposal... *)
-        else (s, {|Packet a (leader_of_bal s (ballot s)) (Fwd v)|})) )"
+  "propose v s nas acceptors \<equiv> let a = id s; leader_bal = (leader_of_bal s (ballot s) nas) 
+    in
+    (if (leader_bal = a \<and> leader s)
+      then do_2a s (Cmd v) acceptors
+      else (if (leader_bal = a)
+        then (s,{}) (* TODO: here we loose the proposal... *)
+        else (s, {Packet a leader_bal (Fwd v)})))"
  
 (* What if the target process is not the leader anymore? TODO: Then let's forward it again. *)
-definition receive_fwd  :: "'v \<Rightarrow> 'v acc_state \<Rightarrow> ('v acc_state \<times> 'v packet fset)" where
-  "receive_fwd v s \<equiv> let a = id s in 
-    (if (leader_of_bal s (ballot s) = a \<and> leader s) then do_2a s (Cmd v) else (s, ({||})))"
+definition receive_fwd  :: "'v \<Rightarrow> 'v acc_state \<Rightarrow> nat \<Rightarrow> acc set \<Rightarrow> ('v acc_state \<times> 'v packet set)" where
+  "receive_fwd v s nas acceptors \<equiv> let a = id s in 
+    (if (leader_of_bal s (ballot s) nas = a \<and> leader s) then do_2a s (Cmd v) acceptors else (s, ({})))"
 
-definition send_1a :: "'v acc_state \<Rightarrow> ('v acc_state \<times> 'v packet fset)" where
+definition send_1a :: "'v acc_state \<Rightarrow> nat \<Rightarrow> acc set \<Rightarrow> ('v acc_state \<times> 'v packet set)" where
   -- {* a tries to become the leader *}
-  "send_1a s \<equiv>
+  "send_1a s nas acceptors \<equiv>
     (let
         a = id s;
-        b = nx_bal a (ballot s) (nr s);
+        b = nx_bal a (ballot s) nas;
         msg_1a = Phase1a a b in
-      (s\<lparr>ballot := Some b\<rparr>, fimage (\<lambda> a2 . Packet a a2 msg_1a) (acceptors s)))"
+      (s\<lparr>ballot := Some b\<rparr>, image (\<lambda> a2 . Packet a a2 msg_1a) acceptors))"
 
-definition receive_1a :: "acc \<Rightarrow> bal \<Rightarrow> 'v acc_state \<Rightarrow> ('v acc_state \<times> 'v packet fset)" where
+definition receive_1a :: "acc \<Rightarrow> bal \<Rightarrow> 'v acc_state \<Rightarrow> ('v acc_state \<times> 'v packet set)" where
   "receive_1a l b s \<equiv>
     (let bal = ballot s; a = id s in
       (if (bal = None \<or> ((the bal) < b))
@@ -205,8 +198,8 @@ definition receive_1a :: "acc \<Rightarrow> bal \<Rightarrow> 'v acc_state \<Rig
             packet = Packet a l msg_1b;
             state = s\<lparr>ballot := Some b\<rparr>
           in
-          (state, {|packet|}))
-       else (s, {||})))"
+          (state, {packet}))
+       else (s, {})))"
 
 definition update_onebs :: 
   "'v acc_state \<Rightarrow> bal \<Rightarrow> acc \<Rightarrow> (inst \<Rightarrow>f ('v cmd \<times> bal) option) \<Rightarrow> 'v acc_state" where
@@ -215,18 +208,20 @@ definition update_onebs ::
   "update_onebs s bal a2 last_vs \<equiv>
     let
       a = id s;
-      combiner = \<lambda> (xs, y) . (if ((a2, y) \<in> set xs) then xs else (a2, y)#xs);
+      combiner = \<lambda> (xs, y) . (if ((a2, y) \<in> xs) then xs else (insert (a2, y) xs));
       pair_map = ($ (onebs s $ bal), last_vs $);
       at_bal = combiner o$ pair_map
     in s\<lparr>onebs := (onebs s)(bal $:= at_bal)\<rparr>"
 
-definition highest_voted :: "(nat \<Rightarrow>f (acc \<times> ('v cmd \<times> nat) option) list) \<Rightarrow> (nat \<Rightarrow>f ('v cmd) option)" where
+definition highest_voted :: "(nat \<Rightarrow>f (acc \<times> ('v cmd \<times> nat) option) set) \<Rightarrow> (nat \<Rightarrow> ('v cmd) option)" where
   -- {* Makes sense only if no list in the map is empty. *}
-  "highest_voted m \<equiv>
+  "highest_voted onebs_bal \<equiv>
     let
-        votes = (map snd) o$ m;
-        highest = (\<lambda> l . if (l = []) then None else (fold max l (l!0)) \<bind> (\<lambda> vb . Some (fst vb)))
-    in highest o$ votes"
+        onebs_i = (\<lambda>i. image (\<lambda>s. snd s) (onebs_bal $ i));
+        (*votes = (map snd) o$ m;*)
+        (*highest = (\<lambda> l . if (l = []) then None else (fold max l (l!0)) \<bind> (\<lambda> vb . Some (fst vb)))*)
+        highest = (\<lambda> l . if (l = {}) then None else (the_elem (Set.filter (\<lambda>le. \<forall>x \<in> l. x \<le> le) l)) \<bind> (\<lambda> vb . Some (fst vb)))
+    in highest o onebs_i"
 
 text {* Instead of trying to define the max as a recursive function, let's use finfun_to_list. *}
 value "((K$ False)(5 $:= True)(4 $:= False)(2 $:= True)) $ (2::int)"
@@ -242,33 +237,34 @@ text {*
 
   For now we propose values to all the instances ever started.
 *}
-definition receive_1b :: "(inst \<Rightarrow>f ('v cmd \<times> bal) option) \<Rightarrow> bal \<Rightarrow> acc \<Rightarrow> 'v acc_state \<Rightarrow> ('v acc_state \<times> 'v packet fset)" where
- "receive_1b last_vs bal a2 s \<equiv> (let a = id s in (
+definition receive_1b :: "(inst \<Rightarrow>f ('v cmd \<times> bal) option) \<Rightarrow> bal \<Rightarrow> acc \<Rightarrow> 'v acc_state \<Rightarrow> nat \<Rightarrow> acc set \<Rightarrow> ('v acc_state \<times> 'v packet set)" where
+ "receive_1b last_vs bal a2 s nas acceptors \<equiv> (let a = id s in (
     if (Some bal = ballot s)
     then
       (let s1 = update_onebs s bal a2 last_vs
-       in (if one_b_quorum_received bal s1 
+       in (if one_b_quorum_received bal s1 nas 
           then (let
-              h = highest_voted (onebs s1 $ bal);
-              max_i = let l = (finfun_to_list (onebs s1 $ bal)) in (if l = [] then 0 else hd (rev l));
+              onebs_bal = onebs s1 $ bal;
+              h = highest_voted onebs_bal;
+              max_i = let l = (finfun_to_list onebs_bal) in (if l = [] then 0 else hd (rev l));
               s2 = s1\<lparr>leader := True\<rparr>;
               maxInst = (next_inst s2);
               (*Modified*)
               s3 = s2\<lparr>next_inst := (if max_i+1 < maxInst then maxInst else max_i+1)\<rparr>;
               twoa_is = [1..<max_i+1];
               (* TODO: the following might traverse all the finfun, which is a problem when there are many instances. *)
-              s4 = fold (\<lambda> i s . s\<lparr>twobs := finfun_update_code (twobs s) i ((twobs s $ i)(bal $:= [a]))\<rparr>) twoa_is s3;
-              msgs = map (\<lambda> i . case h $ i of 
+              s4 = fold (\<lambda> i s . s\<lparr>twobs := finfun_update_code (twobs s) i ((twobs s $ i)(bal $:= {a}))\<rparr>) twoa_is s3;
+              msgs = map (\<lambda> i . case h i of 
                   None \<Rightarrow> Phase2a i bal NoOp a
                 | Some v \<Rightarrow> Phase2a i bal v a) twoa_is;
-              pckts = map (\<lambda> m . send_all s a m) msgs
-            in (s4, fold (op |\<union>|) pckts {||}) )
-          else (s1, {||}) ) )
-    else (s, {||})) )"
+              pckts = map (\<lambda> m . send_all s a m acceptors) msgs
+            in (s4, fold (op \<union>) pckts {}) )
+          else (s1, {}) ) )
+    else (s, {})) )"
 
 definition is_decided where "is_decided s i \<equiv> decided s $ i \<noteq> None"
 
-definition new_twobs where "new_twobs a ori_twobs \<equiv> a # ori_twobs"
+definition new_twobs where "new_twobs a ori_twobs \<equiv> insert a ori_twobs"
 
 definition update_twobs where "update_twobs s i b new \<equiv>
   s\<lparr>twobs := finfun_update_code (twobs s) i (twobs s $ i)(b $:= new)\<rparr>"
@@ -280,21 +276,21 @@ definition update_decided where
         commit_buffer := (commit_buffer s)(i $:= Some v)
 \<rparr>"
 
-definition receive_2_addl  :: "inst \<Rightarrow> bal \<Rightarrow> 'v cmd \<Rightarrow> acc \<Rightarrow> 'v acc_state \<Rightarrow> 'v acc_state" where
- "receive_2_addl i b v l s \<equiv>
+definition receive_2_addl  :: "inst \<Rightarrow> bal \<Rightarrow> 'v cmd \<Rightarrow> acc \<Rightarrow> 'v acc_state \<Rightarrow> nat \<Rightarrow> 'v acc_state" where
+ "receive_2_addl i b v l s nas \<equiv>
     (let a = id s; ori_twobs = (twobs s $ i $ b) in
-    if (l \<in> set ori_twobs) then s 
-     else (let s2 = update_twobs s i b (new_twobs l ori_twobs); votes = (length (twobs s2 $ i $ b))
+    if (l \<in> ori_twobs) then s 
+     else (let s2 = update_twobs s i b (new_twobs l ori_twobs); votes = (card (twobs s2 $ i $ b))
      in (
-          if (2 * votes \<le> nr s) (* Build the quorum *)
+          if (2 * votes \<le> nas) (* Build the quorum *)
           then (
             (s2)
           ) else ( 
-              if ( ((nr s div 2)+1) = votes) (* Decision Time *)
+              if ( ((nas div 2)+1) = votes) (* Decision Time *)
               then ( 
                (update_decided s2 i v)
               ) else ( 
-                  if (nr s = votes) (* Last Message *)
+                  if (nas = votes) (* Last Message *)
                   then ( 
                     let s3= s2\<lparr> working_instances := (working_instances s)(i $:= 2)\<rparr>
                     in (s3)
@@ -304,18 +300,18 @@ definition receive_2_addl  :: "inst \<Rightarrow> bal \<Rightarrow> 'v cmd \<Rig
         ))
     )"     
 
-definition receive_2_first  :: "inst \<Rightarrow> bal \<Rightarrow> 'v cmd \<Rightarrow> acc \<Rightarrow> 'v acc_state \<Rightarrow> 'v acc_state" where
- "receive_2_first i b v l s \<equiv>
+definition receive_2_first  :: "inst \<Rightarrow> bal \<Rightarrow> 'v cmd \<Rightarrow> acc \<Rightarrow> 'v acc_state \<Rightarrow> nat \<Rightarrow> 'v acc_state" where
+ "receive_2_first i b v l s nas \<equiv>
     (let a = id s; bal = (ballot s); s2 = s\<lparr>vote := finfun_update_code (vote s) i (Some v),
-                    twobs := finfun_update_code (twobs s) i ((K$ [])((the bal) $:= [a,l])),
-                    next_inst := i+1,
+                    twobs := finfun_update_code (twobs s) i ((K$ {})((the bal) $:= {a,l})),
+                    next_inst := i + 1,
                     working_instances := (working_instances s)(i $:= 1)\<rparr>
      in (
-          if (3 < nr s)
+          if (3 < nas)
           then ( 
             (s2)
           ) else ( 
-              if (3 = nr s)
+              if (3 = nas)
               then ( 
                 (update_decided s2 i v)
               ) else ( (*nr = 2 *) (*Decided and not working as no more message to receive*)
@@ -328,21 +324,21 @@ definition receive_2_first  :: "inst \<Rightarrow> bal \<Rightarrow> 'v cmd \<Ri
 
 
             
-definition receive_2 :: "inst \<Rightarrow> bal \<Rightarrow> 'v cmd \<Rightarrow> acc \<Rightarrow> 'v acc_state \<Rightarrow> 'v acc_state" where
-  "receive_2 i b v l s \<equiv>
+definition receive_2 :: "inst \<Rightarrow> bal \<Rightarrow> 'v cmd \<Rightarrow> acc \<Rightarrow> 'v acc_state \<Rightarrow> nat \<Rightarrow> 'v acc_state" where
+  "receive_2 i b v l s nas \<equiv>
   (if ((working_instances s) $ i > 0) (* This is not the first message from the instance *)
         then (
-          receive_2_addl i b v l s  
+          receive_2_addl i b v l s nas
       ) else (* This is the first message, treat like a propose *)
      (
-          receive_2_first i b v l s  
+          receive_2_first i b v l s nas
      ))"
 
-definition receive_2a :: "inst \<Rightarrow> bal \<Rightarrow> 'v cmd \<Rightarrow> acc \<Rightarrow> 'v acc_state \<Rightarrow> ('v acc_state \<times> 'v packet fset)" where
-  "receive_2a i b v l s \<equiv> (receive_2 i b v l s, send_all s (id s) (Phase2b i b (id s) v))"
+definition receive_2a :: "inst \<Rightarrow> bal \<Rightarrow> 'v cmd \<Rightarrow> acc \<Rightarrow> 'v acc_state \<Rightarrow> nat \<Rightarrow> acc set \<Rightarrow> ('v acc_state \<times> 'v packet set)" where
+  "receive_2a i b v l s nas acceptors \<equiv> (receive_2 i b v l s nas, send_all s (id s) (Phase2b i b (id s) v) acceptors)"
 
-definition receive_2b :: "inst \<Rightarrow> bal \<Rightarrow> acc \<Rightarrow> 'v cmd  \<Rightarrow> 'v acc_state \<Rightarrow> ('v acc_state \<times> 'v packet fset)" where
-  "receive_2b i b a2 v s \<equiv> (receive_2 i b v a2 s, {||})"
+definition receive_2b :: "inst \<Rightarrow> bal \<Rightarrow> acc \<Rightarrow> 'v cmd  \<Rightarrow> 'v acc_state \<Rightarrow> nat \<Rightarrow> ('v acc_state \<times> 'v packet set)" where
+  "receive_2b i b a2 v s nas \<equiv> (receive_2 i b v a2 s nas, {})"
 
 definition get_last_decision where 
   "get_last_decision s \<equiv> the (decided s $ (the (last_decision s)))"
@@ -350,19 +346,11 @@ definition get_last_decision where
 value "largestprefix [(1,v1), (2,v2), (4,v4)]"
 
 text {* output transition could return an option *}
-definition learn :: "inst \<Rightarrow> 'v  \<Rightarrow> 'v acc_state \<Rightarrow> ('v acc_state \<times> 'v packet fset) option" where 
+definition learn :: "inst \<Rightarrow> 'v  \<Rightarrow> 'v acc_state \<Rightarrow> ('v acc_state \<times> 'v packet set) option" where 
   "learn i v s \<equiv> 
     case (decided s $ i) of None \<Rightarrow> None |
       Some cm \<Rightarrow> (case cm of NoOp \<Rightarrow> None 
-        | Cmd c \<Rightarrow> (if v = c then Some (s, {||}) else None))"
-
-fun process_msg where
-  "process_msg (Phase1a l b) s = receive_1a l b s"
-| "process_msg (Phase1b lvs b a) s = receive_1b lvs b a s"
-| "process_msg (Phase2a i b cm l) s = receive_2a i b cm l s"
-| "process_msg (Phase2b i b a cm) s = receive_2b i b a cm s"
-| "process_msg (Vote i cm) s = undefined"
-| "process_msg (Fwd v) s = receive_fwd v s"
+        | Cmd c \<Rightarrow> (if v = c then Some (s, {}) else None))"
 
 text {* Serializing finfuns to lists *}
 
@@ -372,60 +360,11 @@ definition finfun_filter :: "'a::linorder \<Rightarrow>f 'b \<Rightarrow> 'b \<R
 
 value "let ff = ((K$ 0) :: int \<Rightarrow>f int)(1 $:= 42)(42 $:= 0)(43 $:= 1) in (finfun_filter_v1 ff 0 2) "
 
-subsection {* Internal Handlers *}
-
-datatype 'v internal_event =
-  NoEvent | Commit "'v cmd"
- 
-definition event_handler_get_next_to_commit  :: "'v acc_state \<Rightarrow> ('v acc_state \<times> 'v internal_event) option" where
-  "event_handler_get_next_to_commit s \<equiv> if (((commit_buffer s) $ ((last_committed s)+1)) = None)
-    then None
-    else Some (s\<lparr>last_committed := ((last_committed s)+1), 
-          commit_buffer := ((commit_buffer s)(((last_committed s)+1) $:= None)) \<rparr>, 
-          Commit (the ((commit_buffer s) $ ((last_committed s)+1))))"
-
-fun dequeue :: "'v list \<Rightarrow> (('v list \<times> 'v) option)" where
-"dequeue (a#l) = Some (l, a)" |
-"dequeue [] = None"
-    
-(* This handler performs a snapshot. Considering filtering on onebs as needed. *)
-definition event_handler_process_any_snapshots  :: "'v acc_state \<Rightarrow> 'v acc_state option" where
-  "event_handler_process_any_snapshots s \<equiv> 
-    let sp=(dequeue (snapshot_proposal s))
-    in (
-      if ( sp = None) 
-      then None (* Nothing todo *)
-      else (  
-        if ((snd (the sp)) > (last_committed s))
-        then
-          None  (* we are trying to snapshot but haven't committed that far *)
-        else
-          Some (s\<lparr>snapshot_proposal := (fst (the sp)), snapshot_reference := (snd (the sp)),
-                decided := (finfun_filter (decided s) None (snd (the sp))), 
-                vote := (finfun_filter (vote s) None (snd (the sp))),
-                last_ballot := (finfun_filter (last_ballot s) None (snd (the sp))),
-                twobs := (finfun_filter (twobs s) (K$ []) (snd (the sp)))
-                \<rparr>)
-      )
-    )"
-
-definition propose_snapshot :: "'v acc_state \<Rightarrow> inst \<Rightarrow> 'v acc_state option " where
-  "propose_snapshot s instance \<equiv> 
-    if (instance \<le> (snapshot_reference s)) then 
-       None
-    else ( 
-      let 
-        s2 = s\<lparr>snapshot_proposal := ((snapshot_proposal s) @ [instance]) \<rparr>
-       in
-        Some s2
-    )"
-
-
 section {* The I/O-automata *}
 
 record 'v mp_state = 
   node_states :: "nat \<Rightarrow>f 'v acc_state"
-  network :: "'v packet fset"
+  network :: "'v packet set"
 
 datatype 'v mp_action =
   Receive_fwd acc acc 'v
@@ -442,22 +381,24 @@ locale mp_ioa = IOA +
     -- {* The number of acceptors *}
 begin
 
+definition mp_acclist where "mp_acclist n \<equiv>  (accs n)"
+definition mp_acceptors where "mp_acceptors n \<equiv> (set (mp_acclist n))"
+
 definition mp_asig where
   "mp_asig \<equiv>
-    \<lparr> inputs = { Propose a c | a c . a |\<in>| accs nas},
-      outputs = { Learn l i v | i v l . l |\<in>| accs nas},
-      internals = {Receive_fwd a1 a2 v | a1 a2 v . a1 |\<in>| accs nas \<and> a2 |\<in>| accs nas}
-        \<union> {Send_1as a | a . a |\<in>| accs nas}
-        \<union> {Receive_1a_send_1b a1 a2 b | a1 a2 b . a1 |\<in>| accs nas \<and> a2 |\<in>| accs nas}
-        \<union> {Receive_1b a1 a2 f b | a1 a2 f b . a1 |\<in>| accs nas \<and> a2 |\<in>| accs nas}
-        \<union> {Receive_2a_send_2b a1 a2 i b c | a1 a2 i b c . a1 |\<in>| accs nas \<and> a2 |\<in>| accs nas}
-        \<union> {Receive_2b a1 a2 i b c | a1 a2 i b c. a1 |\<in>| accs nas \<and> a2 |\<in>| accs nas}
-        \<union> {Learn a i c | a i c . a |\<in>| accs nas}\<rparr>"
+    \<lparr> inputs = { Propose a c | a c . a \<in> (mp_acceptors nas)},
+      outputs = { Learn l i v | i v l . l \<in> (mp_acceptors nas)},
+      internals = {Receive_fwd a1 a2 v | a1 a2 v . a1 \<in> (mp_acceptors nas) \<and> a2 \<in> (mp_acceptors nas)}
+        \<union> {Send_1as a | a . a \<in> (mp_acceptors nas)}
+        \<union> {Receive_1a_send_1b a1 a2 b | a1 a2 b . a1 \<in> (mp_acceptors nas) \<and> a2 \<in> (mp_acceptors nas)}
+        \<union> {Receive_1b a1 a2 f b | a1 a2 f b . a1 \<in> (mp_acceptors nas) \<and> a2 \<in> (mp_acceptors nas)}
+        \<union> {Receive_2a_send_2b a1 a2 i b c | a1 a2 i b c . a1 \<in> (mp_acceptors nas) \<and> a2 \<in> (mp_acceptors nas)}
+        \<union> {Receive_2b a1 a2 i b c | a1 a2 i b c. a1 \<in> (mp_acceptors nas) \<and> a2 \<in> (mp_acceptors nas)}
+        \<union> {Learn a i c | a i c . a \<in> (mp_acceptors nas)}\<rparr>"
 
-fun init_nodes_state::"nat \<Rightarrow> nat \<Rightarrow> nat \<Rightarrow>f 'a acc_state" where
-  "init_nodes_state (0::nat) n = (K$ init_acc_state n 0)"
-| "init_nodes_state (Suc i) n = 
-    (if Suc i > n then undefined else (init_nodes_state i n)(i $:= init_acc_state n (i)))"
+fun init_nodes_state::"nat \<Rightarrow> nat \<Rightarrow>f 'a acc_state" where
+  "init_nodes_state (0::nat) = (K$ init_acc_state 0)"
+| "init_nodes_state (Suc i) = (init_nodes_state i)(i $:= init_acc_state (i))"
 
 (*fun init_nodes_state where
   "init_nodes_state (0::nat) n = (K$ init_acc_state n 0)"
@@ -465,81 +406,55 @@ fun init_nodes_state::"nat \<Rightarrow> nat \<Rightarrow> nat \<Rightarrow>f 'a
     (if Suc i > n then undefined else (init_nodes_state i n)(Suc i $:= init_acc_state n (Suc i)))"*)
 
 lemma init_acc: 
-assumes "a < n" and "a \<ge> 0"
-shows "(init_nodes_state (Suc a) n) $ a = init_acc_state n a" using assms
-by (induct a n arbitrary:n rule:init_nodes_state.induct, auto)
-
+assumes "a \<ge> 0"
+shows "(init_nodes_state (Suc a)) $ a = init_acc_state a" using assms
+by (induct a rule:init_nodes_state.induct, auto)
 
 definition mp_start where
-  "mp_start \<equiv> \<lparr>node_states = (init_nodes_state nas nas), network = {||}\<rparr>"
+  "mp_start \<equiv> \<lparr>node_states = (init_nodes_state nas), network = {}\<rparr>"
 
 definition update_state where 
   "update_state a a_s packets s \<equiv>
     s\<lparr>node_states := (node_states s)(a $:= a_s),
-      network := network s |\<union>| packets\<rparr>"
-
-inductive mp_trans where
-  "propose v (node_states s $ a) = (new_s, ps) \<Longrightarrow>
-    mp_trans (s, Propose a (Cmd v), update_state a new_s ps s)"
-| "\<lbrakk>receive_fwd v (node_states s $ dest) = (new_s, ps); 
-    Packet src dest (Fwd v) |\<in>| network s\<rbrakk> \<Longrightarrow>
-      mp_trans (s, Receive_fwd src dest v, update_state a new_s ps s)"
-| "\<lbrakk>receive_1a l b (node_states s $ dest) = (new_s, ps);
-    Packet src dest (Phase1a l b) |\<in>| network s; l = src\<rbrakk> \<Longrightarrow>
-    mp_trans (s, Receive_1a_send_1b src dest b, update_state dest new_s ps s)"
-| "send_1a (node_states s $ l) = (new_s, ps) \<Longrightarrow>
-    mp_trans (s, Send_1as l, update_state l new_s ps s)"
-| "\<lbrakk>receive_1b vs b l (node_states s $ l) = (new_s, ps); 
-    Packet src l (Phase1b vs b a) |\<in>| network s; src = a\<rbrakk> \<Longrightarrow>
-      mp_trans (s, Receive_1b src l vs b, update_state l new_s ps s)"
-| "\<lbrakk>receive_2b i b l cm (node_states s $ l) = (new_s, ps);
-    Packet src l (Phase2b i b a cm) |\<in>| network s; src = a\<rbrakk> \<Longrightarrow>
-      mp_trans (s, Receive_2b a l i b cm, update_state l new_s ps s)"
-| "\<lbrakk>receive_2a i b cm dest (node_states s $ dest) = (new_s, ps);
-    Packet src dest (Phase2a i b cm l) |\<in>| network s; src = l\<rbrakk> \<Longrightarrow>
-      mp_trans (s, Receive_2a_send_2b l dest i b cm, update_state dest new_s ps s)"
-| "learn i v (node_states s $ a) = Some (new_s, ps) \<Longrightarrow>
-    mp_trans (s, Learn a i (Cmd v), update_state a new_s ps s)"
+      network := network s \<union> packets\<rparr>"
 
 fun mp_transit where
-  "mp_transit s (Receive_fwd src dest v) = (if Packet src dest (Fwd v) |\<in>| network s 
-    then (let (new_s, ps) = receive_fwd v (node_states s $ dest) in 
+  "mp_transit s (Receive_fwd src dest v) = (if Packet src dest (Fwd v) \<in> network s 
+    then (let (new_s, ps) = receive_fwd v (node_states s $ dest) nas (mp_acceptors nas) in 
       update_state dest new_s ps s)
     else s)"
-|  "mp_transit s (Propose a (Cmd v)) = (let (new_s, ps) = propose v (node_states s $ a) in
+|  "mp_transit s (Propose a (Cmd v)) = (let (new_s, ps) = propose v (node_states s $ a) nas (mp_acceptors nas) in
     update_state a new_s ps s)" 
-| "mp_transit s (Receive_1a_send_1b src dest b) = (if (Packet src dest (Phase1a src b) |\<in>| network s) 
+| "mp_transit s (Receive_1a_send_1b src dest b) = (if (Packet src dest (Phase1a src b) \<in> network s) 
     then let (new_s, ps) = receive_1a src b (node_states s $ dest) in
       update_state dest new_s ps s 
     else s)"
-| "mp_transit s (Send_1as l) = (let (new_s, ps) = send_1a (node_states s $ l) in
+| "mp_transit s (Send_1as l) = (let (new_s, ps) = send_1a (node_states s $ l) nas (mp_acceptors nas) in
     update_state l new_s ps s)"
-| "mp_transit s (Receive_1b src l vs b) = (if (Packet src l (Phase1b vs b src) |\<in>| network s)
-    then let (new_s, ps) = receive_1b vs b src (node_states s $ l) in
+| "mp_transit s (Receive_1b src l vs b) = (if (Packet src l (Phase1b vs b src) \<in> network s)
+    then let (new_s, ps) = receive_1b vs b src (node_states s $ l) nas (mp_acceptors nas) in
       update_state l new_s ps s 
     else s)"
-| "mp_transit s (Receive_2b a l i b cm) = (if (Packet a l (Phase2b i b a cm) |\<in>| network s)
-    then let (new_s, ps) = receive_2b i b a cm (node_states s $ l) in
+| "mp_transit s (Receive_2b a l i b cm) = (if (Packet a l (Phase2b i b a cm) \<in> network s)
+    then let (new_s, ps) = receive_2b i b a cm (node_states s $ l) nas in
       update_state l new_s ps s 
     else s)"
-| "mp_transit s (Receive_2a_send_2b l dest i b cm) = (if (Packet l dest (Phase2a i b cm l) |\<in>| network s)
-    then (let (new_s, ps) = receive_2a i b cm l (node_states s $ dest) in
+| "mp_transit s (Receive_2a_send_2b l dest i b cm) = (if (Packet l dest (Phase2a i b cm l) \<in> network s)
+    then (let (new_s, ps) = receive_2a i b cm l (node_states s $ dest) nas (mp_acceptors nas) in
         update_state dest new_s ps s)
     else s)"
 | "mp_transit s (Learn a i (Cmd v)) = (case (learn i v (node_states s $ a)) of (Some st) \<Rightarrow> 
   (let (new_s, ps) = st in update_state a new_s ps s)| None \<Rightarrow> s)"
 
-definition mp_ioa where
-  "mp_ioa \<equiv> \<lparr>ioa.asig = mp_asig, start = {mp_start}, trans = {(s,a,t) . mp_trans (s, a, t)}\<rparr>"
-
 end
 
 global_interpretation mp_ioa_3:mp_ioa "3"
-defines mp_start = mp_ioa_3.mp_start and mp_transit = mp_ioa_3.mp_transit
+defines mp_acceptors =  mp_ioa_3.mp_acclist and mp_start = mp_ioa_3.mp_start and mp_transit = mp_ioa_3.mp_transit
 done
 
 definition safe_at::"'v mp_state \<Rightarrow> inst \<Rightarrow> bool" where
-  "safe_at s i \<equiv> (\<forall>acc\<^sub>1 \<in> {0, 1, 2}. \<forall>acc\<^sub>2 \<in> {0, 1, 2}. acc\<^sub>1 \<noteq> acc\<^sub>2 \<longrightarrow>
+  "safe_at s i \<equiv> (let acceptors = set (mp_acceptors 3) in
+    \<forall>acc\<^sub>1 \<in> acceptors. \<forall>acc\<^sub>2 \<in> acceptors. acc\<^sub>1 \<noteq> acc\<^sub>2 \<longrightarrow>
     (case (decided ((node_states s) $ acc\<^sub>1) $ i) of None \<Rightarrow> True |
       Some cm \<Rightarrow> (
         case (decided ((node_states s) $ acc\<^sub>2) $ i) of None \<Rightarrow> True |
@@ -577,6 +492,8 @@ subsection {* Code generation *}
 text {* We need to rename a few modules to let the Scala compiler resolve circular dependencies. *}
 code_identifier
   code_module Code_Numeral \<rightharpoonup> (Scala) MicroCheckerLib
+| code_module Groups \<rightharpoonup> (Scala) MicroCheckerLib
+| code_module Rings \<rightharpoonup> (Scala) MicroCheckerLib
 | code_module Optiona \<rightharpoonup> (Scala) MicroCheckerLib
 | code_module List \<rightharpoonup> (Scala) MicroCheckerLib
 | code_module FinFun \<rightharpoonup> (Scala) MicroCheckerLib
@@ -596,7 +513,7 @@ code_identifier
 | code_module Divides \<rightharpoonup> (Scala) MicroCheckerLib
 | code_module Serialization  \<rightharpoonup> (Scala) MicroCheckerLib
 
-export_code learn send_1a propose process_msg get_last_decision init_acc_state
+export_code learn send_1a propose get_last_decision init_acc_state
   serialize_finfun deserialize_finfun get_ballot is_leader get_leader
 mp_ioa_3.mp_start mp_ioa_3.mp_transit safe_at get_decided ballot_constraint inst_constraint
    in Scala file "MultiPaxos4.scala"
